2D, prob02

Program-proofs/Exercises/2D-counting/prob01/prob01.dfy
@@ -4,7 +4,8 @@
    This is exercise 9.2 from the PC reader
 */
 
-ghost predicate AscDesc(f:(nat,nat) -> int) {
+ghost predicate AscDesc(f:(nat,nat) -> int) 
+{
     // Expresses the property that f is ascending in its first 
     // argument and descending in its second argument, i.e. 
     // ∀ i,j,k ∈ ℕ:
@@ -14,10 +15,10 @@ ghost predicate AscDesc(f:(nat,nat) -> int) {
   (forall i,j,k:: j <= k  ==>  f(i,j) >= f(i,k))
 }
 
-method search2D(h:(nat,nat) -> int, c: int, ghost X: nat, ghost Y: nat) 
+method problem01(h:(nat,nat) -> int, c: int, ghost X: nat, ghost Y: nat)
 returns (x: nat, y: nat)
 requires AscDesc(h) && h(X,Y) == c
-ensures h(x,y) == c
+ensures x <= X && y <= Y && h(x,y) == c 
 {
   /* 
     Given is a function h: ℕ × ℕ → ℤ that is ascending in its 
@@ -29,7 +30,8 @@ ensures h(x,y) == c
     the following specification:
   
       const c: ℤ
-      var x,y: ℤ
+      var   x,y: ℤ
+      
         {P: 0 ≤ X ∧ 0 ≤ Y ∧ h(X,Y) = c}
       T
         {Q: 0 ≤ x ≤ X ∧ 0 ≤ y ≤ Y ∧ h(x,y) = c}
