Program-proofs/Exercises/2D-counting/prob02/prob02.dfy
@@ -1,0 +1,43 @@
+/* file: prob02.dfy
+   author: your name
+   description: extra practice in Dafny, 2D-counting, prob02
+   This is exercise 9.3 from the PC reader
+*/
+
+ghost predicate DescAsc(f:(nat,nat) -> int) 
+{
+    // Expresses the property that f is descending in its first 
+    // argument and ascending in its second argument, i.e. 
+    // ∀ i,j,k ∈ ℕ:
+    //   if i ≤ j then f(i,k) ≥ f(j,k)
+    //   if j ≤ k then f(i,j) ≤ f(i,k)
+  (forall i,j,k:: i <= j  ==>  f(i,k) >= f(j,k)) &&
+  (forall i,j,k:: j <= k  ==>  f(i,j) <= f(i,k))
+}
+
+method problem02(g:(int,int) -> int, m:int, n:int) 
+returns (r: int)
+requires DescAsc(g)
+ensures r == g(m,n)
+{
+  /* 
+    Given is a function g: ℤ × ℤ → ℤ that is descending in its 
+    first argument and ascending in its second argument. We define
+    a function F that counts the number of points (i,j) such that
+    g(i,j) ≤ 0:
+
+      F(g,x,y) = #{ (i,j) | i,j: 0 ≤ i < x ∧ 0 ≤ j < y ∧ g(i,j) ≤ 0 }
+    
+    Derive a command sequence T that satifies the following 
+    specification:
+  
+      const m,n: ℤ
+      var   r: ℤ
+
+        {P: Z = F(g,m,n)}
+      T
+        {Q: r = Z}
+     
+    The time complexity of T should be in O(m + n).
+  */
+}
