Program-proofs/Exercises/2D-counting/prob02/sol02.dfy
@@ -1,0 +1,46 @@
+/* file: sol02.dfy
+   author: David De Potter
+   description: extra practice in Dafny, 2D counting, 
+   solution to prob02
+   This is exercise 9.3 from the PC reader
+*/
+
+ghost predicate DescAsc(f:(int,int) -> int) 
+{
+  (forall i,j,k :: i <= j  ==>  f(i,k) >= f(j,k)) &&
+  (forall i,j,k :: j <= k  ==>  f(i,j) <= f(i,k))
+}
+
+function F(g:(int,int) -> int, x:int, y:int): int
+requires DescAsc(g)
+{   
+  if x <= 0 || y <= 0 then 0
+  else if g(x - 1, y - 1) <= 0 then F(g, x - 1, y) + y
+  else F(g, x, y - 1)
+}
+
+method problem02(g:(int,int) -> int, m:int, n:int) 
+returns (r: int)
+requires DescAsc(g)
+ensures r == F(g, m ,n)
+{
+  var x, y, z := m, n, 0;
+  
+  while x > 0 && y > 0
+    invariant z + F(g, x, y) == F(g, m, n)
+    decreases x + y
+  {
+    if g(x - 1, y - 1) <= 0
+    {
+      z := z + y;
+      x := x - 1;
+    }
+
+    else
+    {
+      y := y - 1;
+    }
+  }
+
+  r := z;
+}
