Program-proofs/Exercises/2D-counting/prob02/sol02Annotated.dfy
@@ -1,0 +1,128 @@
+/* file: sol02Annotated.dfy
+   author: David De Potter
+   description: extra practice in Dafny, 2D counting, 
+   solution to prob02, with annotations
+   This is exercise 9.3 from the PC reader
+*/
+
+ghost predicate DescAsc(f:(int,int) -> int) 
+{
+    // Expresses the property that f is descending in its first 
+    // argument and ascending in its second argument, i.e. 
+    // ∀ i,j,k ∈ ℤ:
+    //   if i ≤ j then f(i,k) ≥ f(j,k)
+    //   if j ≤ k then f(i,j) ≤ f(i,k)
+  (forall i,j,k :: i <= j  ==>  f(i,k) >= f(j,k)) &&
+  (forall i,j,k :: j <= k  ==>  f(i,j) <= f(i,k))
+}
+
+function F(g:(int,int) -> int, x:int, y:int): int
+requires DescAsc(g)
+{   
+    // We define
+    //   F(x,y) = #{ (i,j) | i,j: 0 ≤ i < x ∧ 0 ≤ j < y ∧ g(i,j) ≤ 0 }
+    // This function counts the number of points in the rectangle [0,x) × [0,y) 
+    // that satisfy g(i,j) ≤ 0. 
+    // Base case: x ≤ 0 or y ≤ 0, then the rectangle is empty and F(x,y) = # ∅ = 0.
+    // Recursive case: in this case we want to shrink the rectangle by either
+    //                 decrementing x or y. 
+    //
+    // What happens if we decrement x? 
+    //   F(x,y)
+    //   = #{ (i,j) | i,j: 0 ≤ i < x ∧ 0 ≤ j < y ∧ g(i,j) ≤ 0 }
+    //       ( split domain into 0 ≤ i < x-1 and i = x-1 )
+    //   = #{ (i,j) | i,j: 0 ≤ i < x-1 ∧ 0 ≤ j < y ∧ g(i,j) ≤ 0 }
+    //     + #{ (x-1,j) | j: 0 ≤ j < y ∧ g(x-1,j) ≤ 0 }
+    //       ( apply definition of F to the first term )
+    //   = F(x-1,y) + #{ (x-1,j) | j: 0 ≤ j < y ∧ g(x-1,j) ≤ 0 }
+    //       ( note that the second term counts the number of points in the last column,
+    //         which is determined by the value of g in the rectangle's upper-right 
+    //         corner (x-1,y-1):
+    //         assume g(x-1,y-1) ≤ 0, then since g is ascending in its second argument, 
+    //         g(x-1,y-1) is maximal and we have g(x-1,j) ≤ 0 for all 0 ≤ j < y )
+    //   = F(x - 1,y) + #{ j | j: 0 ≤ j < y }
+    //        ( size of half-open interval [0,y) = y - 0 = y )
+    //   = F(x - 1,y) + y
+    //
+    // What happens if we decrement y?
+    //   F(x,y)
+    //   = #{ (i,j) | i,j: 0 ≤ i < x ∧ 0 ≤ j < y ∧ g(i,j) ≤ 0 }
+    //       ( split domain into 0 ≤ j < y-1 and j = y-1 )
+    //   = #{ (i,j) | i,j: 0 ≤ i < x ∧ 0 ≤ j < y-1 ∧ g(i,j) ≤ 0 }
+    //     + #{ (i,y-1) | i: 0 ≤ i < x ∧ g(i,y-1) ≤ 0 }
+    //       ( apply definition of F to the first term )
+    //   = F(x,y-1) + #{ (i,y-1) | i: 0 ≤ i < x ∧ g(i,y-1) ≤ 0 }
+    //       ( note that the second term counts the number of points in the upper row;
+    //         assume g(x-1,y-1) > 0, then since g is descending in its first argument,
+    //         g(x-1,y-1) is minimal and we have g(i,y-1) > 0 for all 0 ≤ i < x )
+    //   = F(x,y-1) + # ∅
+    //       ( size of empty set is 0 )
+    //   = F(x,y-1)
+
+  if x <= 0 || y <= 0 then 0
+  else if g(x - 1, y - 1) <= 0 then F(g, x - 1, y) + y
+  else F(g, x, y - 1)
+}
+
+method problem02(g:(int,int) -> int, m:int, n:int) 
+returns (r: int)
+requires DescAsc(g)
+ensures r == F(g, m ,n)
+{
+    // Initialization to establish J before the loop
+    // P: F(g,m,n) = Z
+    //   ( arithmetic )
+    // 0 + F(g,m,n) = F(g,m,n)
+  var x, y, z := m, n, 0;
+    // J: z + F(g,x,y) = F(g,m,n)
+
+  while x > 0 && y > 0
+    invariant z + F(g, x, y) == F(g, m, n)
+    decreases x + y
+  {
+      // J ∧ B ∧ vf = V
+      // z + F(g,x,y) = F(g,m,n) ∧ x > 0 ∧ y > 0 ∧ x + y = V
+      //   ( we want to apply the recursive definition of F, so we need 
+      //     to distinguish the cases g(x-1,y-1) ≤ 0 and g(x-1,y-1) > 0 )
+
+    if g(x - 1, y - 1) <= 0
+    {
+        // z + F(g,x,y) = F(g,m,n) ∧ g(x-1,y-1) ≤ 0 ∧ x > 0 ∧ y > 0 ∧ x + y = V
+        //   ( apply definition of F; 
+        //     since x > 0 ∧ y > 0, we are not in the base case )
+        // z + F(g,x-1,y) + y = F(g,m,n) ∧ x + y = V
+      z := z + y;
+        // z + F(g,x-1,y) = F(g,m,n) ∧ x + y = V
+        //    ( prepare for decrementing x )
+        // z + F(g,x-1,y) = F(g,m,n) ∧ x - 1 + y < V
+      x := x - 1;
+        // z + F(g,x,y) = F(g,m,n) ∧ x + y < V
+        // J ∧ vf < V
+    }
+
+    else
+    {
+        // z + F(g,x,y) = F(g,m,n) ∧ g(x-1,y-1) > 0 ∧ x > 0 ∧ y > 0 ∧ x + y = V
+        //   ( apply definition of F; 
+        //     since x > 0 ∧ y > 0, we are not in the base case )
+        // z + F(g,x,y-1) = F(g,m,n) ∧ x + y = V
+        //    ( prepare for decrementing y )
+        // z + F(g,x,y-1) = F(g,m,n) ∧ x + y - 1 < V
+      y := y - 1;
+        // z + F(g,x,y) = F(g,m,n) ∧ x + y < V
+        // J ∧ vf < V
+    }
+
+      // collect branches:
+      // J ∧ vf < V
+  }
+
+    // J ∧ ¬B
+    // z + F(g,x,y) = F(g,m,n) ∧ x ≤ 0 ∨ y ≤ 0
+    //   ( apply base case of F )
+    // z + 0 = F(g,m,n)
+    // z = F(g,m,n)
+  r := z;
+    // r = F(g,m,n)
+    // Q: r = Z
+}
